vera/VerilogEquivalence.v
@@ -18,9 +18,10 @@ From ExtLib Require Import Structures.Monoid.
 From ExtLib Require Import Structures.Traversable.
 From ExtLib Require Import Programming.Show.
 
-Require Import ZArith.
-Require Import String.
-Require Import List.
+From Coq Require Import ZArith.
+From Coq Require Import String.
+From Coq Require Import List.
+From Coq Require Import Sorting.Permutation.
 
 Import ListNotations.
 Import CommonNotations.
@@ -29,57 +30,13 @@ Import FunctorNotation.
 Local Open Scope monad_scope.
 Local Open Scope string.
 
-Section prefixing.
-  Variable prefix : string.
-
-  Definition prefix_name (name : string) : string :=
-    prefix ++ "__" ++ name.
-
-  Equations prefix_names_qfbv : SMT.qfbv string -> SMT.qfbv string := {
-    | SMT.BVVar n => SMT.BVVar (prefix_name n)
-    | SMT.BVOr l r => SMT.BVOr (prefix_names_qfbv l) (prefix_names_qfbv r)
-    | SMT.BVAnd l r => SMT.BVAnd (prefix_names_qfbv l) (prefix_names_qfbv r)
-    | SMT.BVAdd l r => SMT.BVAdd (prefix_names_qfbv l) (prefix_names_qfbv r)
-    | SMT.BVMul l r => SMT.BVMul (prefix_names_qfbv l) (prefix_names_qfbv r)
-    | SMT.BVNeg e => SMT.BVNeg (prefix_names_qfbv e)
-    | SMT.BVNot e => SMT.BVNot (prefix_names_qfbv e)
-    | SMT.BVShl l r => SMT.BVShl (prefix_names_qfbv l) (prefix_names_qfbv r)
-    | SMT.BVLShr l r => SMT.BVLShr (prefix_names_qfbv l) (prefix_names_qfbv r)
-    | SMT.BVLit val => SMT.BVLit val
-    | SMT.BVZeroExtend count e => SMT.BVZeroExtend count (prefix_names_qfbv e)
-    | SMT.BVExtract lo hi e => SMT.BVExtract lo hi (prefix_names_qfbv e)
-    | SMT.BVConcat l r => SMT.BVConcat (prefix_names_qfbv l) (prefix_names_qfbv r)
-    | SMT.CoreEq l r => SMT.CoreEq (prefix_names_qfbv l) (prefix_names_qfbv r)
-    | SMT.CoreNot e => SMT.CoreNot (prefix_names_qfbv e)
-    | SMT.CoreITE cond ifT ifF => SMT.CoreITE (prefix_names_qfbv cond) (prefix_names_qfbv ifT) (prefix_names_qfbv ifF)
-    }.
-
-  Equations prefix_names_formula : SMT.formula string -> SMT.formula string := {
-    | SMT.CDeclare name sort => SMT.CDeclare (prefix_name name) sort
-    | SMT.CEqual l r => SMT.CEqual (prefix_names_qfbv l) (prefix_names_qfbv r)
-    | SMT.CDistinct l r => SMT.CDistinct (prefix_names_qfbv l) (prefix_names_qfbv r)
-    }.
-
-  Definition prefix_names_formulas : list (SMT.formula string) -> list (SMT.formula string) :=
-    List.map prefix_names_formula.
-
-  Definition prefix_names_smt_netlist (smtnl : SMT.smt_netlist string) : SMT.smt_netlist string :=
-    {| SMT.smtnlName := SMT.smtnlName smtnl ;
-      SMT.smtnlPorts := List.map (fun '(name, dir) => (prefix_name name, dir) ) (SMT.smtnlPorts smtnl) ;
-      SMT.smtnlFormulas := List.map prefix_names_formula (SMT.smtnlFormulas smtnl)
-    |}.
-End prefixing.
-
-Definition prefix_pair (prefix_left prefix_right : string): (string * string) -> (string * string) :=
-  fun '(n1, n2) => (prefix_name prefix_left n1, prefix_name prefix_right n2).
-
 Definition mk_equivalence_formulas
-  (input_pairs output_pairs : list (string * string))
+  (inputs outputs : list string)
   (namemap1 namemap2 : StrFunMap.t (nat * SMTLib.sort))
   : sum string (list SMTLib.term) :=
   inputs_same <-
-    mapT (fun '(n1, n2) =>
-            match namemap1 n1, namemap2 n2 return sum string SMTLib.term with
+    mapT (fun n =>
+            match namemap1 n, namemap2 n with
             | Some (smt_name1, SMTLib.Sort_BitVec size1),
               Some (smt_name2, SMTLib.Sort_BitVec size2) =>
                 if (size1 =? size2)%N
@@ -88,11 +45,11 @@ Definition mk_equivalence_formulas
                             (SMTLib.Term_Fun (smt_name2, ([], SMTLib.Sort_BitVec size2)) []))
                 else inl "err"%string
             | _, _ => inl "err"%string
-            end) input_pairs;;
+            end) inputs;;
   outputs_different <-
     mapT (
-        fun '(n1, n2) =>
-          match namemap1 n1, namemap2 n2 return sum string SMTLib.term with
+        fun n =>
+          match namemap1 n, namemap2 n return sum string SMTLib.term with
           | Some (smt_name1, SMTLib.Sort_BitVec size1),
             Some (smt_name2, SMTLib.Sort_BitVec size2) =>
               if (size1 =? size2)%N
@@ -101,25 +58,37 @@ Definition mk_equivalence_formulas
                                            (SMTLib.Term_Fun (smt_name2, ([], SMTLib.Sort_BitVec size2)) [])))
               else inl "err"%string
           | _, _ => inl "err"%string
-          end) output_pairs;;
+          end) outputs;;
   ret (app inputs_same outputs_different)
 .
 
-Definition equivalence_query
-  (input_pairs output_pairs : list (string * string))
-  (verilog1 verilog2 : Verilog.vmodule)
-  : sum string SMT.smtlib_query :=
+Axiom dec_permutation : forall (l1 l2 : list string), { Permutation l1 l2 } + { ~ Permutation l1 l2 }.
 
-  VerilogTypecheck.tc_vmodule verilog1 ;;
-  VerilogTypecheck.tc_vmodule verilog2 ;;
+Definition assert_dec {P E} (dec : { P } + { ~ P }) (err : E) : sum E P :=
+  match dec with
+  | left prf => inr prf
+  | right _  => inl err
+  end
+.
 
-  canonical_verilog1 <- VerilogCanonicalize.canonicalize_verilog verilog1 ;;
-  canonical_verilog2 <- VerilogCanonicalize.canonicalize_verilog verilog2 ;;
+Definition equivalence_query_canonical
+  (canonical_verilog1 canonical_verilog2 : Verilog.vmodule)
+  : sum string (SMT.smtlib_query) :=
+
+  inputs_ok1 <- assert_dec
+                 (list_eq_dec string_dec (Verilog.inputs canonical_verilog1) (Verilog.inputs canonical_verilog2))
+                 "Inputs don't match" ;;
+
+  outputs_ok2 <- assert_dec
+                 (list_eq_dec string_dec (Verilog.outputs canonical_verilog1) (Verilog.outputs canonical_verilog2))
+                 "Outputs don't match" ;;
 
   query1 <- VerilogToSMT.verilog_to_smt 0 canonical_verilog1 ;;
   query2 <- VerilogToSMT.verilog_to_smt (1 + SMT.max_var query1) canonical_verilog2 ;;
-  equivalence_formulas <- mk_equivalence_formulas input_pairs output_pairs
-                           (SMT.nameVerilogToSMT query1) (SMT.nameVerilogToSMT query2) ;;
+  equivalence_formulas <-
+    mk_equivalence_formulas
+      (Verilog.inputs canonical_verilog1) (Verilog.outputs canonical_verilog1)
+      (SMT.nameVerilogToSMT query1) (SMT.nameVerilogToSMT query2) ;;
 
   ret {|
       SMT.nameSMTToVerilog :=
@@ -133,4 +102,17 @@ Definition equivalence_query
       SMT.declarations := SMT.declarations query1 ++ SMT.declarations query2;
       SMT.assertions := SMT.assertions query1 ++ SMT.assertions query2 ++ equivalence_formulas
     |}
+.
+
+Definition equivalence_query (verilog1 verilog2 : Verilog.vmodule) : sum string SMT.smtlib_query :=
+  VerilogTypecheck.tc_vmodule verilog1 ;;
+  VerilogTypecheck.tc_vmodule verilog2 ;;
+
+  inputs_ok1 <- assert_dec (list_eq_dec string_dec (Verilog.inputs verilog1) (Verilog.inputs verilog2)) "Inputs don't match" ;;
+  outputs_ok2 <- assert_dec (list_eq_dec string_dec (Verilog.outputs verilog1) (Verilog.outputs verilog2)) "Outputs don't match" ;;
+
+  canonical_verilog1 <- VerilogCanonicalize.canonicalize_verilog verilog1 ;;
+  canonical_verilog2 <- VerilogCanonicalize.canonicalize_verilog verilog2 ;;
+
+  equivalence_query_canonical canonical_verilog1 canonical_verilog2
 .
