vera/VerilogEquivalenceCorrectness.v
@@ -12,6 +12,7 @@ From vera Require Import Tactics.
 Import VerilogSemantics.CombinationalOnly.
 
 From Coq Require Import Relations.
+From Coq Require Import Sorting.Permutation.
 
 From Equations Require Import Equations.
 From ExtLib Require Import Structures.Monads.
@@ -24,44 +25,45 @@ Require Import String.
 From Coq Require Import List.
 Import ListNotations.
 Import EqNotations.
+Local Open Scope string.
+Local Open Scope Z_scope.
 
 Definition match_on_regs
-  (regs : list (string * string))
+  (regs : list string)
   (v1 v2 : VerilogState)
   : Prop :=
   List.Forall
-    (fun '(n1, n2) =>
-       exists v, regState v1 n1 = Some v
-            /\ regState v2 n2 = Some v
+    (fun 'n =>
+       exists v, regState v1 n = Some v
+            /\ regState v2 n = Some v
             /\ ~ XBV.has_x v
     ) regs.
 
-Definition equivalent
-  (inputs outputs : list (string * string))
-  (v1 v2 : Verilog.vmodule)
-  : Prop :=
+Definition no_errors (v : Verilog.vmodule) :=
   forall (input_vals : list XBV.t)
-    (input_len_ok : length input_vals = length inputs)
-    (input_vals_defined : Forall (fun bv => ~ XBV.has_x bv) input_vals)
-    (final1 final2 : VerilogState),
-    let init1 :=
-      set_regs (List.map
-                  (fun '((n, _), v) => (n, v))
-                  (List.combine inputs input_vals))
-        (initial_state v1)
-    in
-    let init2 :=
-      set_regs (List.map
-                  (fun '((_, n), v) => (n, v))
-                  (List.combine inputs input_vals))
-        (initial_state v2)
-    in
-    multistep_eval init1 final1 ->
-    multistep_eval init2 final2 ->
-    match_on_regs outputs final1 final2
-.
+    (input_len_ok : length input_vals = length (Verilog.inputs v))
+    (input_vals_defined : Forall (fun bv => ~ XBV.has_x bv) input_vals),
+    let init := set_regs (List.combine (Verilog.inputs v) input_vals) (initial_state v) in
+    exists final, multistep_eval init final.
 
-Local Open Scope string.
+Record equivalent (v1 v2 : Verilog.vmodule) : Prop :=
+  MkEquivalent {
+      interface_inputs_match : Verilog.inputs v1 = Verilog.inputs v2;
+      interface_outputs_match : Verilog.outputs v1 = Verilog.outputs v2;
+      no_errors1 : no_errors v1;
+      no_errors2 : no_errors v2;
+      behaviour_match :
+      forall (input_vals : list XBV.t)
+        (input_len_ok : length input_vals = length (Verilog.inputs v1))
+        (input_vals_defined : Forall (fun bv => ~ XBV.has_x bv) input_vals)
+        (final1 final2 : VerilogState),
+        let init1 := set_regs (List.combine (Verilog.inputs v1) input_vals) (initial_state v1) in
+        let init2 := set_regs (List.combine (Verilog.inputs v1) input_vals) (initial_state v2) in
+        multistep_eval init1 final1 ->
+        multistep_eval init2 final2 ->
+        match_on_regs (Verilog.outputs v1) final1 final2;
+    }
+.
 
 Section V.
   Import Verilog.
@@ -100,85 +102,45 @@ Section V.
     |}.
 End V.
 
-#[local] Open Scope Z_scope.
-
-Example assign_out_equivalent : equivalent [("in", "in")] [("out", "out")] assign_out assign_out.
+Example assign_out_equivalent : equivalent assign_out assign_out.
 Proof.
-  unfold equivalent, match_on_regs.
-  intros * ? ? * [eval1 blocked1] [eval2 blocked2].
-  simpl in input_len_ok.
-  repeat (destruct input_vals; try solve [simpl in *; discriminate]).
-  repeat (destruct input_vals_defined; try solve [simpl in *; discriminate]).
-  simpl in *.
-  unfold assign_out, set_reg in eval1; simpl in eval1.
-  unfold assign_out, set_reg in eval2; simpl in eval2.
-  repeat constructor.
-  unfold multistep_eval, multistep in *.
-  eapply clos_trans_t1n in eval1; inversion eval1 as [ ? step1 | ? ? step1_1 step1_2 ]; subst;
-    repeat (unfold step in *; simp run_step exec_module_item exec_statement eval_expr in *; simpl in * );
-    unfold set_reg in *; simpl in *; try solve_by_inverts 3%nat.
-  eapply clos_trans_t1n in eval2.
-  inversion eval2 as [ ? step2 | ? ? step2_1 step2_2 ]; subst;
-    repeat (unfold step in *; simp run_step exec_module_item exec_statement eval_expr in *; simpl in * );
-    unfold set_reg in *; simpl in *; try solve_by_inverts 3%nat.
-  inv step1.
-  inv step2.
-  eexists. intuition.
+  constructor; try auto.
+  - unfold no_errors. intros.
+    repeat (destruct input_vals; try solve [simpl in *; discriminate]).
+    eexists.
+    repeat (unfold no_errors, assign_out, set_reg, initial_state; simpl).
+    repeat (try econstructor; try unfold step; simpl; try simp run_step exec_module_item exec_statement).
+  - unfold no_errors. intros.
+    repeat (destruct input_vals; try solve [simpl in *; discriminate]).
+    repeat (unfold no_errors, assign_out, set_reg, initial_state; simpl).
+    eexists.
+    repeat (try econstructor; try unfold step; simpl; try simp run_step exec_module_item exec_statement).
+  - unfold match_on_regs.
+    intros * ? ? * [eval1 blocked1] [eval2 blocked2].
+    simpl in input_len_ok.
+    repeat (destruct input_vals; try solve [simpl in *; discriminate]).
+    repeat (destruct input_vals_defined; try solve [simpl in *; discriminate]).
+    simpl in *.
+    unfold assign_out, set_reg in eval1; simpl in eval1.
+    unfold assign_out, set_reg in eval2; simpl in eval2.
+    repeat constructor.
+    unfold multistep_eval, multistep in *.
+    eapply clos_trans_t1n in eval1; inversion eval1 as [ ? step1 | ? ? step1_1 step1_2 ]; subst;
+      repeat (unfold step in *; simp run_step exec_module_item exec_statement eval_expr in *; simpl in * );
+      unfold set_reg in *; simpl in *; try solve_by_inverts 3%nat.
+    eapply clos_trans_t1n in eval2.
+    inversion eval2 as [ ? step2 | ? ? step2_1 step2_2 ]; subst;
+      repeat (unfold step in *; simp run_step exec_module_item exec_statement eval_expr in *; simpl in * );
+      unfold set_reg in *; simpl in *; try solve_by_inverts 3%nat.
+    inv step1.
+    inv step2.
+    eexists. intuition.
 Qed.
-
-Example assign_out_twostep_equivalent : equivalent [("in", "in")] [("out", "out")] assign_out assign_out_twostep.
-Proof.
-  unfold equivalent, match_on_regs.
-  intros * ? ? * [eval1 blocked1] [eval2 blocked2].
-  simpl in input_len_ok.
-  repeat (destruct input_vals_defined; try solve [simpl in *; discriminate]).
-  simpl in *.
-  (* unfold assign_out, set_reg in eval1; simpl in eval1. *)
-  (* unfold assign_out, set_reg in eval2; simpl in eval2. *)
-  repeat constructor.
-  unfold multistep_eval, multistep in *.
-  eapply clos_trans_t1n in eval1; inversion eval1 as [ ? step1 | ? ? step1_1 step1_2 ]; subst;
-    repeat (unfold step in *; simp run_step exec_module_item exec_statement eval_expr in *; simpl in * );
-    unfold set_reg in *; simpl in *; try solve_by_inverts 3%nat.
-  inv step1.
-  eapply clos_trans_t1n in eval2; inversion eval2 as [ ? step2 | ? ? step2_1 step2_2 ]; subst;
-    repeat (unfold step in *; simp run_step exec_module_item exec_statement eval_expr in *; simpl in * );
-    unfold set_reg in *; simpl in *; try solve_by_inverts 3%nat.
-  inv step2_1.
-  inversion step2_2 as [ ? step2_2' | ? ? step2_2' step2_3 ]; subst;
-    repeat (unfold step in *; simp run_step exec_module_item exec_statement eval_expr in *; simpl in * );
-    unfold set_reg in *; simpl in *; try solve_by_inverts 3%nat.
-  inv step2_2'.
-  eexists. simpl.
-  intuition. f_equal.
-Admitted.
-
-Definition inputs (v : Verilog.vmodule) : list string :=
-  map_opt (fun p => match p with
-                 | {|
-                     Verilog.portDirection := PortIn;
-                     Verilog.portName := name
-                   |} => Some name
-                 | _ => None
-                 end)
-    (Verilog.modPorts v).
-
-Definition outputs (v : Verilog.vmodule) : list string :=
-  map_opt (fun p => match p with
-                 | {|
-                     Verilog.portDirection := PortOut;
-                     Verilog.portName := name
-                   |} => Some name
-                 | _ => None
-                 end)
-    (Verilog.modPorts v).
 
 Theorem canonicalize_correct v v' :
   VerilogCanonicalize.canonicalize_verilog v = inr v' ->
-  equivalent (List.map dupe (inputs v)) (List.map dupe (outputs v)) v v'.
+  equivalent v v'.
 Admitted.
-
-Compute SMTLib.interp_fun_type SMT.no_uninterp_sorts [] (SMTLib.Sort_BitVec 5).
 
 Definition match_on_regs_smt
   (regs : list string)
@@ -200,13 +162,13 @@ Definition match_verilog_model
   (m : SMT.model SMT.no_uninterp_sorts)
   : Prop :=
   forall (input_vals : list XBV.t)
-    (input_len_ok : length input_vals = length (inputs v))
+    (input_len_ok : length input_vals = length (Verilog.inputs v))
     (input_vals_defined : Forall (fun bv => ~ XBV.has_x bv) input_vals)
     (final : VerilogState),
-    let init := set_regs (List.combine (inputs v) input_vals) (initial_state v) in
+    let init := set_regs (List.combine (Verilog.inputs v) input_vals) (initial_state v) in
     multistep_eval init final ->
-    match_on_regs_smt (inputs v) nameMap init m ->
-    match_on_regs_smt (outputs v) nameMap final m
+    match_on_regs_smt (Verilog.inputs v) nameMap init m ->
+    match_on_regs_smt (Verilog.outputs v) nameMap final m
 .
 
 Theorem verilog_to_smt_correct start v q :
@@ -216,10 +178,99 @@ Theorem verilog_to_smt_correct start v q :
   match_verilog_model (SMT.nameVerilogToSMT q) v model.
 Admitted.
 
-Theorem equivalence_query_correct input_pairs output_pairs verilog1 verilog2 query :
-  equivalence_query input_pairs output_pairs verilog1 verilog2 = inr query ->
+Theorem equivalence_query_canonical_correct verilog1 verilog2 query :
+  equivalence_query_canonical verilog1 verilog2 = inr query ->
   SMT.unsat query ->
-  equivalent input_pairs output_pairs verilog1 verilog2.
+  equivalent verilog1 verilog2.
+Admitted.
+
+Lemma match_on_regs_trans :
+  forall rs v1 v2 v3,
+    match_on_regs rs v1 v2 ->
+    match_on_regs rs v2 v3 ->
+    match_on_regs rs v1 v3.
+Proof.
+  intro rs.
+  induction rs; unfold match_on_regs.
+  - constructor.
+  - intros * H1 H2.
+    rewrite Forall_forall in *.
+    intros x Hin.
+    destruct (H1 ltac:(assumption) ltac:(assumption)) as [val1 ?].
+    destruct (H2 ltac:(assumption) ltac:(assumption)) as [val2 ?].
+    exists val1.
+    intuition congruence.
+Qed.
+
+Lemma match_on_regs_sym :
+  forall rs v1 v2,
+    match_on_regs rs v1 v2 ->
+    match_on_regs rs v2 v1.
+Proof.
+  intro rs.
+  induction rs; unfold match_on_regs.
+  - constructor.
+  - intros * H.
+    rewrite Forall_forall in *.
+    intros x Hin.
+    destruct (H ltac:(assumption) ltac:(assumption)) as [val ?].
+    exists val.
+    intuition congruence.
+Qed.
+
+Lemma equivalent_trans v1 v2 v3 :
+  equivalent v1 v2 ->
+  equivalent v2 v3 ->
+  equivalent v1 v3.
+Proof.
+  intros [interface_inputs_match1 interface_outputs_match1 no_errors1 no_errors2 behaviour_match1].
+  intros [interface_inputs_match2 interface_outputs_match2 _ no_errors3 behaviour_match2].
+  constructor; simpl in *.
+  all: (try rewrite <- interface_inputs_match2 in *;
+        try rewrite <- interface_inputs_match1 in *;
+        try rewrite <- interface_outputs_match2 in *;
+        try rewrite <- interface_outputs_match1 in *;
+        simpl in *
+       ).
+  - congruence.
+  - congruence.
+  - assumption.
+  - assumption.
+  - intros.
+    specialize (behaviour_match1 input_vals ltac:(assumption) ltac:(assumption)).
+    specialize (behaviour_match2 input_vals ltac:(assumption) ltac:(assumption)).
+    assert (exists final', multistep_eval (set_regs (combine (Verilog.inputs v1) input_vals) (initial_state v2)) final') as H1. {
+      unfold no_errors in *.
+      rewrite <- interface_inputs_match2 in *.
+      rewrite <- interface_inputs_match1 in *.
+      simpl in *.
+      eauto.
+    }
+    destruct H1.
+    eapply match_on_regs_trans; eauto.
+Qed.
+
+Lemma equivalent_sym v1 v2 :
+  equivalent v1 v2 ->
+  equivalent v2 v1.
+Proof.
+  intros [interface_inputs_match1 interface_outputs_match1 no_errors1 no_errors2 behaviour_match1].
+  constructor.
+  - congruence.
+  - congruence.
+  - assumption.
+  - assumption.
+  - simpl in *. intros.
+    rewrite <- interface_outputs_match1 in *.
+    rewrite <- interface_inputs_match1 in *.
+    apply match_on_regs_sym.
+    eauto.
+Qed.
+
+Theorem equivalence_query_correct verilog1 verilog2 query :
+  equivalence_query verilog1 verilog2 = inr query ->
+  SMT.unsat query ->
+  equivalent verilog1 verilog2.
 Proof.
   intros Hquery Hunsat.
   unfold equivalence_query in *.
@@ -237,5 +288,7 @@ Proof.
          | [ H : VerilogToSMT.verilog_to_smt _ _ = inr _ |- _ ] =>
              pose proof (verilog_to_smt_correct _ _ _ H); clear H
          end.
-  (* Owl goes here *)
-Admitted.
+  intuition eauto using equivalent_trans, equivalent_sym, equivalence_query_canonical_correct.
+Qed.
+
+Print Assumptions equivalence_query_correct.
